Define full funs interp, in middle of proofs
Proved In for single and full, funsym version
In middle of proving NoDup, injectivity issue with names
Added badvars everywhere to ensure uniqueness

proofs/transform/eliminate_algebraic.v
@@ -133,7 +133,12 @@ Definition funsym_clone (f: funsym) (n: string) : funsym :=
 (*Should it be funsym -> string or string -> string?*)
 Variable (new_constr_name: funsym -> string).
 
-Definition new_constr (f: funsym) : funsym := funsym_clone f (new_constr_name f).
+(*We need to make sure new funsym names are unique*)
+Variable badnames: list string.
+
+Definition gen_id s := gen_name s badnames.
+
+Definition new_constr (f: funsym) : funsym := funsym_clone f (gen_id (new_constr_name f)).
 
 (*Parameterize by no_ind, no_inv, no_sel*)
 (*Ignore no_sel and no_inv - not used anywhere*)
@@ -211,7 +216,7 @@ Proof.
 Qed.
 
 Definition selector_funsym(ts: typesym) (csl: list funsym) : funsym :=
-  let mt_id : string := ("match_" ++ ts_name ts)%string in
+  let mt_id : string := gen_id ("match_" ++ ts_name ts)%string in
   let mt_var := gen_name "a" (ts_args ts) in
   let mt_ty : vty := vty_var mt_var in
   let ty := vty_cons ts (map vty_var (ts_args ts)) in
@@ -231,7 +236,7 @@ Definition selector_axiom
   (*fix ty*)
   let ty := vty_cons ts (map vty_var (ts_args ts)) in
   (* declare the selector function *)
-  let mt_id : string := ("match_" ++ ts_name ts)%string in
+  let mt_id : string := gen_id ("match_" ++ ts_name ts)%string in
   (*TODO: does it need to be fresh? Yes, cannot be in params of ts*)
   let mt_var := gen_name "a" (ts_args ts) in
   let mt_ty : vty := vty_var mt_var in
@@ -319,7 +324,7 @@ Qed.
 (*Again, will prove nodup does nothing*)
 Definition indexer_funsym (ts: typesym) : funsym :=
   let ty := vty_cons ts (map vty_var (ts_args ts)) in
-  let mt_id := ("index_" ++ (ts_name ts))%string in
+  let mt_id := gen_id ("index_" ++ (ts_name ts))%string in
   Build_funsym (Build_fpsym mt_id (nodup typevar_eq_dec (ts_args ts)) [ty] 
     (indexer_check_args ts) (nodupb_nodup _ _)) vty_int false 0 eq_refl.
 
@@ -328,7 +333,7 @@ Definition indexer_funsym (ts: typesym) : funsym :=
 Definition indexer_axiom
   (ts: typesym) (*(ty : vty)*) (csl : list funsym) : funsym * list (string * formula) :=
   (* declare the indexer function *)
-  let mt_id := ("index_" ++ (ts_name ts))%string in
+  let mt_id := gen_id ("index_" ++ (ts_name ts))%string in
   let mt_ls := indexer_funsym ts in (*funsym_noconstr_noty mt_id [ty] vty_int in*)
   (* define the indexer function *)
   let mt_add idx (cs: funsym) :=
@@ -372,7 +377,7 @@ Fixpoint map_pairs {A B: Type} (f: A -> A -> B) (l: list A) : list B :=
 Definition discriminator_axioms (ts: typesym) (ty: vty) (csl: list funsym) : 
   list (string * formula) :=
   let d_add (c1: funsym) (c2: funsym) : (string * formula) :=
-    let i : string := ((s_name c1) ++ "_" ++ (s_name c2))%string in
+    let i : string := gen_id ((s_name c1) ++ "_" ++ (s_name c2))%string in
     (* let pr = create_prsymbol (id_derive id ts.ts_name) in *)
     (*Create vars - TODO: does it have to be fresh against some vars?*)
     let ul := rev (combine (gen_names (length (s_args c1)) "u" nil) (s_args c1)) in
@@ -456,7 +461,7 @@ Definition proj_funsym (c: funsym) (n: string) (ty: vty) (Hty: In ty (s_args c))
 
 Definition projection_syms (c: funsym) : list funsym :=
   let conv_p (i: nat) (ty: vty) (Hty: In ty (s_args c)) :=
-    let id := ((s_name c) ++ "_proj_" ++ (nat_to_string i))%string in
+    let id := gen_id ((s_name c) ++ "_proj_" ++ (nat_to_string i))%string in
     proj_funsym c id ty Hty
     (* TODO: do we need option?(funsym_noconstr_noty id [f_ret c] ty) *)
   in
